% Options for packages loaded elsewhere
\PassOptionsToPackage{unicode}{hyperref}
\PassOptionsToPackage{hyphens}{url}
%
\documentclass[
]{article}
\usepackage{amsmath,amssymb}
\usepackage{lmodern}
\usepackage{ifxetex,ifluatex}
\ifnum 0\ifxetex 1\fi\ifluatex 1\fi=0 % if pdftex
  \usepackage[T1]{fontenc}
  \usepackage[utf8]{inputenc}
  \usepackage{textcomp} % provide euro and other symbols
\else % if luatex or xetex
  \usepackage{unicode-math}
  \defaultfontfeatures{Scale=MatchLowercase}
  \defaultfontfeatures[\rmfamily]{Ligatures=TeX,Scale=1}
\fi
% Use upquote if available, for straight quotes in verbatim environments
\IfFileExists{upquote.sty}{\usepackage{upquote}}{}
\IfFileExists{microtype.sty}{% use microtype if available
  \usepackage[]{microtype}
  \UseMicrotypeSet[protrusion]{basicmath} % disable protrusion for tt fonts
}{}
\makeatletter
\@ifundefined{KOMAClassName}{% if non-KOMA class
  \IfFileExists{parskip.sty}{%
    \usepackage{parskip}
  }{% else
    \setlength{\parindent}{0pt}
    \setlength{\parskip}{6pt plus 2pt minus 1pt}}
}{% if KOMA class
  \KOMAoptions{parskip=half}}
\makeatother
\usepackage{xcolor}
\IfFileExists{xurl.sty}{\usepackage{xurl}}{} % add URL line breaks if available
\IfFileExists{bookmark.sty}{\usepackage{bookmark}}{\usepackage{hyperref}}
\hypersetup{
  pdftitle={FCDs},
  pdfauthor={Daniel Dennis},
  hidelinks,
  pdfcreator={LaTeX via pandoc}}
\urlstyle{same} % disable monospaced font for URLs
\usepackage[margin=1in]{geometry}
\usepackage{graphicx}
\makeatletter
\def\maxwidth{\ifdim\Gin@nat@width>\linewidth\linewidth\else\Gin@nat@width\fi}
\def\maxheight{\ifdim\Gin@nat@height>\textheight\textheight\else\Gin@nat@height\fi}
\makeatother
% Scale images if necessary, so that they will not overflow the page
% margins by default, and it is still possible to overwrite the defaults
% using explicit options in \includegraphics[width, height, ...]{}
\setkeys{Gin}{width=\maxwidth,height=\maxheight,keepaspectratio}
% Set default figure placement to htbp
\makeatletter
\def\fps@figure{htbp}
\makeatother
\setlength{\emergencystretch}{3em} % prevent overfull lines
\providecommand{\tightlist}{%
  \setlength{\itemsep}{0pt}\setlength{\parskip}{0pt}}
\setcounter{secnumdepth}{-\maxdimen} % remove section numbering
-\usepackage{amsmath}
\ifluatex
  \usepackage{selnolig}  % disable illegal ligatures
\fi

\title{FCDs}
\author{Daniel Dennis}
\date{09/06/2021}

\begin{document}
\maketitle

\[p(\boldsymbol{y},\boldsymbol{s}|\mu_1,...,\mu_k,\sigma_1^2,...,\sigma^2_K,\xi)=p(\boldsymbol{y}|\boldsymbol{s},\mu_1,...,\mu_k,\sigma_1^2,...,\sigma^2_K)p(\boldsymbol{s}|\xi)\]
where \[
p(\boldsymbol{y}|\boldsymbol{s},\mu_1,...,\mu_k,\sigma_1^2,...,\sigma^2_K)=p(y_1|s_1=s_1,\mu_{s_1},\sigma^2_{s_1})\times p(y_2|s_2=s_2,\mu_{s_2},\sigma^2_{s_2})\times...\times p(y_T|s_T,\mu_{s_T},\sigma^2_{s_T})\\
\begin{aligned}
&=\prod^K_{k=1}\prod_{t:s_t=k}p(y_t|s_t=k,\mu_k,\sigma^2_k)\\
&=\prod^K_{k=1}\prod_{t:s_t=k}\frac{1}{\sqrt{2\pi\sigma^2_k}}exp \left\{-\frac{1}{2\sigma^2_k}(y_t-\mu_k)^2\right\}\\
&\propto\prod^K_{k=1}\sigma^{2\left(-\frac{N_k}{2}\right)}_k exp\left\{-\frac{1}{2\sigma^2_k}\sum_{t:s_t=k}(y_t-\mu_k)^2\right\}
\end{aligned}
\] where \(N_k\) is the number of observations in state k.

The full conditional distribution for \(\mu_1,...,\mu_k\) is therefore:
\[
\pi(\mu_1,...,\mu_K|\boldsymbol{y},\boldsymbol{s},\sigma^2_1,...,\sigma^2_K,\xi)\propto p(\boldsymbol{y},\boldsymbol{s}|\mu_1,...,\mu_k,\sigma^2_1,...,\sigma^2_K,\xi) \pi(\mu_1,...,\mu_K)\\
\]

\$\$

\begin{aligned}

& =p(\boldsymbol{y}|\boldsymbol{s},\mu_1,...,\mu_k,\sigma^2_1,...,\sigma^2_K)p(\boldsymbol{s}|\xi)\pi(\mu_1,...,\mu_K)\\

& \propto p(\boldsymbol{y}|\boldsymbol{s},\mu_1,...,\mu_k,\sigma^2_1,...,\sigma^2_K)\pi(\mu_1,...,\mu_K)\\

& =p(\boldsymbol{y}|\boldsymbol{s},\mu_1,...,\mu_k,\sigma^2_1,...,\sigma^2_K)\times \prod^K_{k=1}\pi(\mu_k)\\

\end{aligned}

\textbackslash{}

\begin{aligned}\\

&\propto\prod^K_{k=1}\sigma_k^{2\left(-\frac{N_k}{2}\right)}exp\left\{-\frac{1}{2\sigma^2_k}\sum_{t:s_t=k}(y_t-\mu_k)^2\right\}\times\prod^K_{k=1}exp\left\{-\frac{1}{2v}(\mu_k-m)^2\right\}\\

&\propto\prod^K_{k=1}exp\left\{-\frac{1}{2\sigma^2_k}\left(\sum_{t:s_t=k}(y_t^2-2y_t\mu_k+\mu_k^2)\right)-\frac{1}{2v}(\mu_k-m)^2\right\}\\

&=\prod^K_{k=1}exp\left\{-\frac{1}{2\sigma^2_k}\left(\sum_{t:s_t=k}y_t^2-2\mu_k\sum_{t:s_t=k}y_t+\mu_k^2\sum_{t:s_t=k}1\right)-\frac{1}{2v}(\mu_k^2-2\mu_km+m^2)\right\}\\

&=\prod^K_{k=1}exp\left\{-\frac{1}{2\sigma^2_k}\left(\sum_{t:s_t=k}y_t^2-2\mu_kN_k\bar{y}_k+N_k\mu_k^2\right)-\frac{1}{2v}(\mu_k^2-2\mu_km+m^2)\right\}\\

&\propto\prod^K_{k=1}exp\left\{-\frac{1}{2\sigma^2_k}(-2\mu_kN_k\bar{y}_k+N_k\mu_k^2)-\frac{1}{2v}(\mu_k^2-2\mu_km)\right\}\\

&=\prod^K_{k=1}exp\left\{-\frac{1}{2\sigma^2_kv}(v[-2\mu_kN_k\bar{y}_k+N_k\mu_k^2])+\sigma^2_k(\mu_k^2-2\mu_km)\right\}\\

&=\prod^K_{k=1}exp\left\{-\frac{1}{2\sigma^2_kv}([vN_k+\sigma^2_k]\mu_k^2-2\mu_kN_k\bar{y}_kv-2\mu_km\sigma^2_k)\right\}\\

&=\prod^K_{k=1}exp\left\{-\frac{1}{\frac{2\sigma^2_kv}{vN_k+\sigma^2_k}}\left[
\mu_k^2-2\left(\frac{vN_k\bar{y}_k+\sigma^2_km}{vN_k+\sigma^2_k}\right)\mu_k\right]\right\}\\

&=\prod^K_{k=1}exp\left\{-\frac{1}{\frac{2\sigma^2_kv}{vN_k+\sigma^2_k}}\left[
\left(\mu_k-\frac{vN_k\bar{y}_k+\sigma^2_km}{vN_k+\sigma^2_k}\right)^2-\left(
\frac{vN_k\bar{y}_k+\sigma^2_km}{vN_k+\sigma^2_k}
\right)^2\right]\right\}\\

&\propto\prod^K_{k=1}exp\left\{-\frac{vN_k+\sigma^2_k}{2\sigma^2_kv}\left[
\left(\mu_k-\frac{vN_k\bar{y}_k+\sigma^2_km}{vN_k+\sigma^2_k}\right)^2\right]\right\}\\

\end{aligned}

\[
So, because this factorises as a product of densities for $\mu_1,...,\mu_K$, the $\mu_k$ are independent in the full conditional distribution with
\]\mu\_k\textbar{}\boldsymbol{y},\boldsymbol{s},\sigma\^{}2\_k,\xi\sim N\left(
\frac{vN_k\bar{y}_k+\sigma^2_km}{vN_k+\sigma^2_k},\frac{\sigma^2_kv}{vN_k+\sigma^2_k}\right)\$\$

where \(\bar{y}_k=\frac{1}{N_k}\sum_{t:s_t=k}y_t\) for \(k=1,...,K\).

The full conditional distribution for \(\sigma^2_1,...,\sigma^2_K\) is:

\$\$
\pi(\sigma\textsuperscript{2\_1,\ldots,\sigma}2\_K\textbar{}\boldsymbol{y},\boldsymbol{s},\mu\_1,\ldots,\mu\_K,\xi)\propto p(\boldsymbol{y},\boldsymbol{s}\textbar{}\mu\_1,\ldots,\mu\_k,\sigma\textsuperscript{2\_1,\ldots,\sigma}2\_K,\xi)\pi(\sigma\textsuperscript{2\_1,\ldots,\sigma}2\_K)\textbackslash{}

\begin{aligned}

& =p(\boldsymbol{y}|\boldsymbol{s},\mu_1,...,\mu_k,\sigma^2_1,...,\sigma^2_K)p(\boldsymbol{s}|\xi)\pi(\sigma^2_1,...,\sigma^2_K)\\

& \propto p(\boldsymbol{y}|\boldsymbol{s},\mu_1,...,\mu_k,\sigma^2_1,...,\sigma^2_K)\pi(\sigma^2_1,...,\sigma^2_K)\\

& =p(\boldsymbol{y}|\boldsymbol{s},\mu_1,...,\mu_k,\sigma^2_1,...,\sigma^2_K)\times \prod^K_{k=1}\pi(\sigma^2_k)\\

\end{aligned}

\textbackslash{}

\begin{aligned}\\

&=\prod^K_{k=1}\sigma_k^{2\left(-\frac{N_k}{2}\right)}exp\left\{-\frac{1}{2\sigma^2_k}\sum_{t:s_t=k}(y_t-\mu_k)^2\right\}\times
\prod^K_{k=1}\frac{\beta}{\Gamma(\alpha)}\sigma^{2(-\alpha-1)}_kexp\left\{-\frac{\beta}{\sigma^2_k}\right\}\\

&\propto\prod^K_{k=1}\sigma_k^{2\left(-\alpha-\frac{N_k}{2}-1\right)}exp\left\{-\frac{1}{2\sigma^2_k}\left(\sum_{t:s_t=k}(y_t-\mu_k)^2\right)-\frac{\beta}{\sigma^2_k}\right\}\\

&=\prod^K_{k=1}\sigma_k^{2\left(-\alpha-\frac{N_k}{2}-1\right)}exp\left\{-\frac{1}{\sigma^2_k}\left(\beta+\sum_{t:s_t=k}\frac{(y_t-\mu_k)^2}{2}\right)\right\}\\
\end{aligned}

\textbackslash{} \$\$

So, we can see that \(\sigma^2_k\) is independent in its full
conditional distributions and that \[
\sigma^2_k|\boldsymbol{y},\boldsymbol{s},\mu_k,\xi\sim invgamma\left(\alpha+\frac{N_k}{2},\beta+\sum_{t:s_t=k}\frac{(y_t-\mu_k)^2}{2}\right)
\]

\end{document}
